src/program_proof/memkv/erpc_proof.v
@@ -5,6 +5,10 @@ From Perennial.base_logic Require Import lib.ghost_map lib.mono_nat lib.saved_sp
 From Perennial.program_proof Require Import grove_prelude std_proof marshal_stateless_proof.
 From Perennial.program_proof.memkv Require Import urpc_proof urpc_spec erpc_lib.
 
+Notation erpcG Σ := (erpc_lib.erpcG Σ (list u8)).
+
+Definition erpcN := nroot .@ "erpc".
+
 (** Spec for an eRPC handler.
 This is isomorphic to uRPCSpec, but to avoid confusion we use distinct types. *)
 Record eRPCSpec {Σ} :=
@@ -13,8 +17,8 @@ Record eRPCSpec {Σ} :=
     espec_Pre : espec_ty → list u8 → iProp Σ;
     espec_Post : espec_ty → list u8 → list u8 → iProp Σ }.
 
-Section erpc.
-Context `{rpcG Σ (list u8), invGS Σ}.
+Section erpc_defs.
+Context `{!erpcG Σ, !urpcregG Σ, !gooseGlobalGS Σ}.
 
 Local Definition encode_request (rid : RPCRequestID) (payload : list u8) :=
   u64_le rid.(Req_CID) ++ u64_le rid.(Req_Seq) ++ payload.
@@ -23,12 +27,12 @@ Local Definition encode_request (rid : RPCRequestID) (payload : list u8) :=
     we compute the spec of the underlying uRPC handler. *)
 Definition eRPCSpec_uRPC γrpc (spec : eRPCSpec (Σ:=Σ)) : uRPCSpec :=
  {| spec_rpcid := spec.(espec_rpcid);
-    spec_ty := rpc_request_names * RPCRequestID * (list u8) * spec.(espec_ty);
+    spec_ty := erpc_request_names * RPCRequestID * (list u8) * spec.(espec_ty);
     spec_Pre :=(λ '(γreq, rid, payload, x) req,
-                  ⌜req = encode_request rid payload⌝ ∗
+                  ⌜req = encode_request rid payload ∧ int.Z rid.(Req_Seq) > 0⌝ ∗
                   is_RPCRequest γrpc γreq
-                     (spec.(espec_Pre) x req)
-                     (spec.(espec_Post) x req)
+                     (spec.(espec_Pre) x payload)
+                     (spec.(espec_Post) x payload)
                      rid
              )%I;
     spec_Post :=(λ '(γreq, rid, payload, x) req rep,
@@ -38,7 +42,250 @@ Definition eRPCSpec_uRPC γrpc (spec : eRPCSpec (Σ:=Σ)) : uRPCSpec :=
  |}.
 
 (** Convenience function to say that a given rpcid has such a handler *)
-Definition handler_erpc_spec`{!urpcregG Σ, !gooseGlobalGS Σ} Γsrv γrpc (host:u64) (spec : eRPCSpec) :=
+Definition handler_erpc_spec `{!urpcregG Σ} Γsrv γrpc (host:u64) (spec : eRPCSpec) :=
   handler_urpc_spec Γsrv host (eRPCSpec_uRPC γrpc spec).
 
-End erpc.
+End erpc_defs.
+
+Section erpc_proof.
+
+Context `{hG: !heapGS Σ}.
+Context `{!urpcregG Σ, !erpcG Σ}.
+
+Definition own_erpc_server (s : loc) (γ : erpc_names) : iProp Σ :=
+  ∃ (lastReply_ptr lastSeq_ptr:loc)
+    (lastReplyM:gmap u64 (list u8)) (lastReplyMV:gmap u64 goose_lang.val)
+    (lastSeqM:gmap u64 u64) (nextCID:u64),
+  "HlastReply" ∷ s ↦[erpc.Server :: "lastReply"] #lastReply_ptr ∗
+  "HlastReplyMap" ∷ map.is_map lastReply_ptr 1 (lastReplyMV, zero_val (slice.T byteT)) ∗ (* TODO: default *)
+  "%HlastReplyMVdom" ∷ ⌜dom (gset u64) lastReplyMV = dom (gset u64) lastSeqM⌝ ∗
+  "HlastReply_structs" ∷ ([∗ map] k ↦ v;rep ∈ lastReplyMV ; lastReplyM,
+    ∃ val_sl q, ⌜v = slice_val val_sl⌝ ∗ typed_slice.is_slice_small val_sl byteT q rep) ∗
+  "HlastSeq" ∷ s ↦[erpc.Server :: "lastSeq"] #lastSeq_ptr ∗
+  "HlastSeqMap" ∷ is_map lastSeq_ptr 1 lastSeqM ∗
+  "HnextCID" ∷ s ↦[erpc.Server :: "nextCID"] #nextCID ∗
+  "Herpc" ∷ RPCServer_own_ghost γ lastSeqM lastReplyM ∗
+  "Hcids" ∷ [∗ set] cid ∈ (fin_to_set u64), ⌜int.Z cid < int.Z nextCID⌝%Z ∨ (is_eRPCClient_ghost γ cid 1)
+.
+
+Definition is_erpc_server (s:loc) γ : iProp Σ :=
+  ∃ mu (cm:loc),
+  "#His_srv" ∷ is_RPCServer γ ∗
+  "#Hmu" ∷ readonly (s ↦[erpc.Server :: "mu"] mu) ∗
+  "#HmuInv" ∷ is_lock erpcN mu (own_erpc_server s γ)
+.
+
+Definition impl_erpc_handler_spec (f : val) (spec : eRPCSpec)
+   : iProp Σ :=
+  ∀ (x : spec.(espec_ty)) (reqData : list u8) req rep dummy_rep_sl dummy,
+  {{{
+    is_slice_small req byteT 1 reqData ∗
+    rep ↦[slice.T byteT] (slice_val dummy_rep_sl) ∗
+    is_slice (V:=u8) dummy_rep_sl byteT 1 dummy ∗
+    spec.(espec_Pre) x reqData
+  }}}
+    f (slice_val req) #rep
+  {{{ rep_sl q repData, RET #();
+      rep ↦[slice.T byteT] (slice_val rep_sl) ∗
+      is_slice_small rep_sl byteT q repData ∗
+      spec.(espec_Post) x reqData repData
+  }}}.
+
+Lemma wp_erpc_Server_HandleRequest spec γ s f :
+  impl_erpc_handler_spec f spec -∗
+  {{{ is_erpc_server s γ }}}
+    Server__HandleRequest #s f
+  {{{ f', RET f'; impl_handler_spec f' (uRPCSpec_Spec $ eRPCSpec_uRPC γ spec) }}}.
+Proof.
+  iIntros "#Hf %Φ !# #Hs HΦ". wp_call. iModIntro.
+  iApply "HΦ". clear Φ.
+  iIntros (reqData Post req repptr ?? Φ) "!# Hpre HΦ". wp_lam.
+  iDestruct "Hpre" as "(Hreq & Hrepptr & Hrep & Hpre)".
+  iSimpl in "Hpre". iDestruct "Hpre" as ([[[γreq rid] payload] x]) "[[[-> %Hseqpos] #HreqInv] Hpost]".
+
+  wp_apply (wp_ReadInt with "Hreq"). clear req.
+  iIntros (req) "Hreq".
+  wp_apply (wp_ReadInt with "Hreq"). clear req.
+  iIntros (req) "Hreq".
+  wp_pures.
+
+  iNamed "Hs".
+  wp_loadField.
+  wp_apply (acquire_spec with "HmuInv").
+  iIntros "[Hlocked Hown]". iNamed "Hown".
+
+  wp_loadField.
+  wp_apply (wp_MapGet with "HlastSeqMap").
+  iIntros (seqno ok) "[%HseqGet HlastSeqMap]".
+  wp_pures.
+
+  wp_apply (wp_and_pure ok (int.Z rid.(Req_Seq) ≤ int.Z seqno)%Z).
+  { wp_pures. iPureIntro. by destruct ok. }
+  { iIntros "_". wp_pures. iPureIntro. done. }
+
+  case_bool_decide as Hif.
+  - (* we hit the reply table *)
+    wp_loadField.
+    wp_apply (map.wp_MapGet with "HlastReplyMap").
+    iIntros (reply replyOk) "[%HlookupReply HlastReplyMap]".
+    wp_pures.
+
+    destruct ok; last first.
+    { exfalso. naive_solver. }
+    apply map_get_true in HseqGet.
+    destruct Hif as [_ HseqLe].
+
+    (* get a copy of the is_slice for the slice we're giving in reply *)
+    assert (is_Some (lastReplyMV !! rid.(Req_CID))) as [xx HlastReplyMVlookup].
+    {
+      assert (rid.(Req_CID) ∈ dom (gset u64) lastSeqM).
+      { by eapply elem_of_dom_2. }
+      assert (rid.(Req_CID) ∈ dom (gset u64) lastReplyMV).
+      { rewrite -HlastReplyMVdom in H. done. }
+      apply elem_of_dom.
+      done.
+    }
+
+    iDestruct (big_sepM2_lookup_iff with "HlastReply_structs") as %Hdom.
+    assert (is_Some (lastReplyM !! rid.(Req_CID))) as [? HlastReplyMlookup].
+    { apply Hdom. naive_solver. }
+
+    iDestruct (big_sepM2_lookup_acc _ _ _ rid.(Req_CID) with "HlastReply_structs") as "[HlastReply_struct HlastReply_structs]".
+    { done. }
+    { done. }
+
+    iDestruct "HlastReply_struct" as (srv_val_sl ?) "[%Hxx Hsrv_val_sl]".
+    assert (xx = reply) as ->.
+    {
+      unfold map.map_get in HlookupReply.
+      rewrite HlastReplyMVlookup in HlookupReply.
+      naive_solver.
+    }
+
+    subst reply.
+    iDestruct "Hsrv_val_sl" as "[Hsrv_val_sl Hrep_val_sl]".
+    iSpecialize ("HlastReply_structs" with "[Hsrv_val_sl]").
+    {
+      iExists _, _.
+      iFrame.
+      done.
+    }
+    wp_store.
+
+    (* now split into stale/nonstale cases *)
+    destruct (Z.lt_ge_cases (int.Z rid.(Req_Seq)) (int.Z seqno)) as [Hcase|Hcase].
+    { (* Stale *)
+      iMod (smaller_seqno_stale_fact _ rid seqno with "His_srv Herpc") as "HH".
+      { done. }
+      { done. }
+      { done. }
+      iDestruct "HH" as "[Hrpc #Hstale]".
+      wp_loadField.
+      wp_apply (release_spec with "[-HΦ Hrep_val_sl Hrepptr Hpost]").
+      {
+        iFrame "#∗".
+        iNext.
+        iExists _,_,_, _, _, _.
+        iFrame.
+        done.
+      }
+      wp_pures. iApply "HΦ". iModIntro.
+      iFrame "Hrep_val_sl Hrepptr".
+      iApply "Hpost". by iLeft.
+    }
+    { (* Not stale *)
+      assert (seqno = rid.(Req_Seq)) as -> by word.
+      iMod (server_replies_to_request _ rid with "His_srv Herpc") as "HH".
+      { done. }
+      { done. }
+      { eexists []. naive_solver. }
+
+      iDestruct "HH" as "[#Hreceipt Hrpc]".
+
+      (* prove that rid.(Req_CID) is in lastReplyMV (probably just add [∗ map] _ ↦ _;_ ∈ lastReplyMV ; lastSeq, True) *)
+      wp_loadField.
+      wp_apply (release_spec with "[-HΦ Hrep_val_sl Hrepptr Hpost]").
+      {
+        iFrame "#∗".
+        iNext.
+        iExists _,_,_, _, _, _.
+        iFrame.
+        done.
+      }
+      wp_pures. iModIntro. iApply "HΦ".
+      iFrame "Hrep_val_sl Hrepptr".
+      iApply "Hpost".
+      iRight.
+      rewrite HlastReplyMlookup.
+      done.
+    }
+  - (* we have to call the handler *)
+    assert (int.Z seqno < int.Z rid.(Req_Seq))%Z as HseqFresh.
+    {
+      simpl.
+      destruct ok.
+      {
+        intuition.
+        destruct (Z.le_gt_cases (int.Z rid.(Req_Seq)) (int.Z seqno)) as [Hineq|Hineq].
+        { naive_solver. }
+        { naive_solver. }
+      }
+      {
+        apply map_get_false in HseqGet as [_ ->].
+        simpl.
+        word.
+      }
+    }
+
+    (* get resources out of escrow *)
+    iMod (server_takes_request with "HreqInv Herpc") as "HH".
+    { done. }
+    { rewrite HseqGet //. }
+    iDestruct "HH" as "(Hγpre & Hpre & Hproc)".
+
+    (* *Now* we reduce the if, which takes a step. And call the handler. *)
+    wp_apply ("Hf" with "[$Hreq $Hrepptr $Hrep $Hpre]").
+    iIntros (rep_sl q rep) "(Hrepptr & Hrep & Hspecpost)".
+
+    wp_loadField.
+    wp_apply (wp_MapInsert with "HlastSeqMap").
+    { done. }
+    iIntros "HlastSeqMap".
+    wp_load.
+    wp_loadField.
+    wp_apply (map.wp_MapInsert with "HlastReplyMap").
+    iIntros "HlastReplyMap".
+    wp_pures.
+
+    iMod (server_completes_request with "His_srv HreqInv Hγpre Hspecpost Hproc") as "HH".
+    { done. }
+    { done. }
+    { rewrite HseqGet. simpl. done. }
+    iDestruct "HH" as "(#Hreceipt & Hrpc)".
+
+    wp_loadField.
+    iDestruct "Hrep" as "[Hrep1 Hrep2]".
+    wp_apply (release_spec with "[-HΦ Hrep1 Hrepptr Hpost]").
+    {
+      iFrame "HmuInv Hlocked".
+      iNext.
+      iExists _,_,_, _, _, _.
+      iFrame.
+      iSplitR.
+      {
+        iPureIntro.
+        simpl.
+        rewrite !dom_insert_L.
+        congruence.
+      }
+      iApply (big_sepM2_insert_2 with "[Hrep2] HlastReply_structs").
+      simpl.
+      iExists _, _.
+      iSplitR; first done.
+      done.
+    }
+    wp_pures. iApply "HΦ". iFrame.
+    iApply "Hpost". iModIntro. iRight. done.
+Qed.
+
+End erpc_proof.
