src/program_proof/memkv/memkv_move_shard_proof.v
@@ -4,7 +4,7 @@ From Perennial.program_proof.memkv Require Export memkv_shard_definitions memkv_
 
 Section memkv_move_shard_proof.
 
-Context `{!heapGS Σ, rpcG Σ ShardReplyC, urpcregG Σ, kvMapG Σ}.
+Context `{!heapGS Σ, erpcG Σ ShardReplyC, urpcregG Σ, kvMapG Σ}.
 
 Lemma wp_MoveShardRPC (s args_ptr:loc) args γsh γ :
   is_KVShardServer s γ -∗
